rocq/Ender/PublicParser.v
@@ -91,7 +91,7 @@ Definition parse_arc (text : PChars) : option ArcName :=
   | _ => None
   end.
 
-Definition parse_public_statement_chars (text : PChars) : option PublicStatement :=
+Definition parse_public_statement_chars_generic (text : PChars) : option PublicStatement :=
   match parse_call text with
   | None => None
   | Some (name, args) =>
@@ -148,14 +148,103 @@ Definition parse_public_statement_chars (text : PChars) : option PublicStatement
     if named "con_arc" then match args with [a;b] => match parse_arc a,parse_arc b with Some A,Some B=>Some(ConArc A B)|_,_=>None end|_=>None end else None
   end.
 
+(** A direct decoder for canonical renderings.  Besides making the common path
+    cheaper, this gives the completeness proof a small structural round trip;
+    the generic call parser remains the fallback for diagnostics and evolution. *)
+Definition parse_rendered_statement (x : PChars) : option PublicStatement :=
+  match x with
+  | ["o"%char;"n"%char;"_"%char;"l"%char;"i"%char;"n"%char;"e"%char;"("%char;a;b;","%char;p;")"%char] => Some (OnLine (segment_name a b) p)
+  | ["t"%char;"r"%char;"a"%char;"n"%char;"s"%char;"v"%char;"e"%char;"r"%char;"s"%char;"a"%char;"l"%char;"("%char;a;","%char;b;","%char;t1;","%char;i1;","%char;c;","%char;d;","%char;t2;","%char;i2;")"%char] => Some (Transversal a b t1 i1 c d t2 i2)
+  | ["i"%char;"n"%char;"t"%char;"e"%char;"r"%char;"s"%char;"e"%char;"c"%char;"t"%char;"_"%char;"s"%char;"e"%char;"g"%char;"("%char;a;b;","%char;c;d;","%char;p;")"%char] => Some (IntersectSeg (segment_name a b) (segment_name c d) p)
+  | ["t"%char;"r"%char;"a"%char;"p"%char;"e"%char;"z"%char;"o"%char;"i"%char;"d"%char;"_"%char;"p"%char;"r"%char;"e"%char;"m"%char;"i"%char;"s"%char;"e"%char;"("%char;"q"%char;"_"%char;a;b;c;d;","%char;e;f;","%char;g;h;")"%char] => Some (TrapezoidPremise (quadrilateral_name a b c d) (segment_name e f) (segment_name g h))
+  | ["k"%char;"i"%char;"t"%char;"e"%char;"_"%char;"p"%char;"r"%char;"e"%char;"m"%char;"i"%char;"s"%char;"e"%char;"("%char;"q"%char;"_"%char;a;b;c;d;","%char;"a"%char;"_"%char;e;f;g;","%char;"a"%char;"_"%char;h;i;j;")"%char] => Some (KitePremise (quadrilateral_name a b c d) (angle_name e f g) (angle_name h i j))
+  | ["i"%char;"s"%char;"o"%char;"s"%char;"_"%char;"t"%char;"r"%char;"a"%char;"p"%char;"e"%char;"z"%char;"o"%char;"i"%char;"d"%char;"_"%char;"p"%char;"r"%char;"e"%char;"m"%char;"i"%char;"s"%char;"e"%char;"("%char;"q"%char;"_"%char;a;b;c;d;","%char;e;f;","%char;g;h;")"%char] => Some (IsosTrapezoidPremise (quadrilateral_name a b c d) (segment_name e f) (segment_name g h))
+  | ["r"%char;"i"%char;"g"%char;"h"%char;"t"%char;"("%char;"a"%char;"_"%char;a;b;c;")"%char] => Some (Right (angle_name a b c))
+  | ["c"%char;"o"%char;"n"%char;"_"%char;"s"%char;"e"%char;"g"%char;"("%char;a;b;","%char;c;d;")"%char] => Some (ConSeg (segment_name a b) (segment_name c d))
+  | ["c"%char;"o"%char;"n"%char;"_"%char;"a"%char;"n"%char;"g"%char;"("%char;"a"%char;"_"%char;a;b;c;","%char;"a"%char;"_"%char;d;e;f;")"%char] => Some (ConAng (angle_name a b c) (angle_name d e f))
+  | ["c"%char;"o"%char;"n"%char;"_"%char;"t"%char;"r"%char;"i"%char;"("%char;"t"%char;"_"%char;a;b;c;","%char;"t"%char;"_"%char;d;e;f;")"%char] => Some (ConTri (triangle_name a b c) (triangle_name d e f))
+  | ["c"%char;"o"%char;"n"%char;"_"%char;"r"%char;"i"%char;"g"%char;"h"%char;"t"%char;"("%char;"a"%char;"_"%char;a;b;c;","%char;"a"%char;"_"%char;d;e;f;")"%char] => Some (ConRight (angle_name a b c) (angle_name d e f))
+  | ["p"%char;"a"%char;"r"%char;"a"%char;"("%char;a;b;","%char;c;d;")"%char] => Some (Para (segment_name a b) (segment_name c d))
+  | ["i"%char;"s"%char;"o"%char;"s"%char;"c"%char;"e"%char;"l"%char;"e"%char;"s"%char;"("%char;"t"%char;"_"%char;a;b;c;")"%char] => Some (Isosceles (triangle_name a b c))
+  | ["p"%char;"e"%char;"r"%char;"p"%char;"("%char;a;b;","%char;c;d;","%char;p;")"%char] => Some (Perp (segment_name a b) (segment_name c d) p)
+  | ["m"%char;"i"%char;"d"%char;"p"%char;"t"%char;"("%char;a;b;","%char;p;")"%char] => Some (Midpt (segment_name a b) p)
+  | ["a"%char;"n"%char;"g"%char;"_"%char;"b"%char;"i"%char;"s"%char;"e"%char;"c"%char;"t"%char;"("%char;"a"%char;"_"%char;a;b;c;","%char;d;e;")"%char] => Some (AngBisect (angle_name a b c) (segment_name d e))
+  | ["r"%char;"e"%char;"c"%char;"t"%char;"a"%char;"n"%char;"g"%char;"l"%char;"e"%char;"("%char;"q"%char;"_"%char;a;b;c;d;")"%char] => Some (Rectangle (quadrilateral_name a b c d))
+  | ["p"%char;"a"%char;"r"%char;"a"%char;"l"%char;"l"%char;"e"%char;"l"%char;"o"%char;"g"%char;"r"%char;"a"%char;"m"%char;"("%char;"q"%char;"_"%char;a;b;c;d;")"%char] => Some (Parallelogram (quadrilateral_name a b c d))
+  | ["p"%char;"r"%char;"o"%char;"p"%char;"o"%char;"r"%char;"t"%char;"i"%char;"o"%char;"n"%char;"("%char;a;b;","%char;c;d;","%char;e;f;","%char;g;h;")"%char] => Some (Proportion (segment_name a b) (segment_name c d) (segment_name e f) (segment_name g h))
+  | ["s"%char;"i"%char;"m"%char;"_"%char;"t"%char;"r"%char;"i"%char;"("%char;"t"%char;"_"%char;a;b;c;","%char;"t"%char;"_"%char;d;e;f;")"%char] => Some (SimTri (triangle_name a b c) (triangle_name d e f))
+  | ["e"%char;"q"%char;"u"%char;"i"%char;"l"%char;"a"%char;"t"%char;"e"%char;"r"%char;"a"%char;"l"%char;"("%char;"t"%char;"_"%char;a;b;c;")"%char] => Some (Equilateral (triangle_name a b c))
+  | ["s"%char;"u"%char;"p"%char;"p"%char;"l"%char;"e"%char;"m"%char;"e"%char;"n"%char;"t"%char;"a"%char;"r"%char;"y"%char;"("%char;"a"%char;"_"%char;a;b;c;","%char;"a"%char;"_"%char;d;e;f;")"%char] => Some (Supplementary (angle_name a b c) (angle_name d e f))
+  | ["c"%char;"o"%char;"m"%char;"p"%char;"l"%char;"e"%char;"m"%char;"e"%char;"n"%char;"t"%char;"a"%char;"r"%char;"y"%char;"("%char;"a"%char;"_"%char;a;b;c;","%char;"a"%char;"_"%char;d;e;f;")"%char] => Some (Complementary (angle_name a b c) (angle_name d e f))
+  | ["l"%char;"i"%char;"n"%char;"e"%char;"a"%char;"r"%char;"_"%char;"p"%char;"a"%char;"i"%char;"r"%char;"("%char;"a"%char;"_"%char;a;b;c;","%char;"a"%char;"_"%char;d;e;f;")"%char] => Some (LinearPair (angle_name a b c) (angle_name d e f))
+  | ["e"%char;"q"%char;"u"%char;"i"%char;"a"%char;"n"%char;"g"%char;"u"%char;"l"%char;"a"%char;"r"%char;"("%char;"t"%char;"_"%char;a;b;c;")"%char] => Some (Equiangular (triangle_name a b c))
+  | ["c"%char;"i"%char;"r"%char;"c"%char;"u"%char;"m"%char;"c"%char;"e"%char;"n"%char;"t"%char;"e"%char;"r"%char;"("%char;p;","%char;"t"%char;"_"%char;a;b;c;")"%char] => Some (Circumcenter p (triangle_name a b c))
+  | ["i"%char;"n"%char;"c"%char;"e"%char;"n"%char;"t"%char;"e"%char;"r"%char;"("%char;p;","%char;"t"%char;"_"%char;a;b;c;")"%char] => Some (Incenter p (triangle_name a b c))
+  | ["p"%char;"e"%char;"r"%char;"p"%char;"_"%char;"b"%char;"i"%char;"s"%char;"e"%char;"c"%char;"t"%char;"o"%char;"r"%char;"("%char;a;b;","%char;c;d;","%char;p;")"%char] => Some (PerpBisector (segment_name a b) (segment_name c d) p)
+  | ["s"%char;"e"%char;"g"%char;"_"%char;"b"%char;"i"%char;"s"%char;"e"%char;"c"%char;"t"%char;"("%char;a;b;","%char;c;d;","%char;p;")"%char] => Some (SegBisect (segment_name a b) (segment_name c d) p)
+  | ["i"%char;"s"%char;"o"%char;"s"%char;"_"%char;"t"%char;"r"%char;"a"%char;"p"%char;"e"%char;"z"%char;"o"%char;"i"%char;"d"%char;"("%char;"q"%char;"_"%char;a;b;c;d;")"%char] => Some (IsosTrapezoid (quadrilateral_name a b c d))
+  | ["r"%char;"h"%char;"o"%char;"m"%char;"b"%char;"u"%char;"s"%char;"("%char;"q"%char;"_"%char;a;b;c;d;")"%char] => Some (Rhombus (quadrilateral_name a b c d))
+  | ["t"%char;"a"%char;"n"%char;"g"%char;"e"%char;"n"%char;"t"%char;"("%char;"c"%char;"_"%char;o;r;","%char;a;b;","%char;p;")"%char] => Some (Tangent (circle_name o r) (segment_name a b) p)
+  | ["c"%char;"h"%char;"o"%char;"r"%char;"d"%char;"("%char;"c"%char;"_"%char;o;r;","%char;a;b;")"%char] => Some (Chord (circle_name o r) (segment_name a b))
+  | ["m"%char;"i"%char;"n"%char;"o"%char;"r"%char;"_"%char;"a"%char;"r"%char;"c"%char;"("%char;"c"%char;"_"%char;o;r;","%char;a;","%char;b;")"%char] => Some (ArcStatement (arc_name MinorArc (circle_name o r) a b))
+  | ["m"%char;"a"%char;"j"%char;"o"%char;"r"%char;"_"%char;"a"%char;"r"%char;"c"%char;"("%char;"c"%char;"_"%char;o;r;","%char;a;","%char;b;")"%char] => Some (ArcStatement (arc_name MajorArc (circle_name o r) a b))
+  | ["r"%char;"a"%char;"d"%char;"i"%char;"u"%char;"s"%char;"("%char;"c"%char;"_"%char;o;r;","%char;p;")"%char] => Some (Radius (circle_name o r) p)
+  | ["d"%char;"i"%char;"a"%char;"m"%char;"e"%char;"t"%char;"e"%char;"r"%char;"("%char;"c"%char;"_"%char;o;r;","%char;a;b;")"%char] => Some (Diameter (circle_name o r) (segment_name a b))
+  | ["i"%char;"n"%char;"s"%char;"c"%char;"r"%char;"i"%char;"b"%char;"e"%char;"d"%char;"_"%char;"a"%char;"n"%char;"g"%char;"l"%char;"e"%char;"("%char;"c"%char;"_"%char;o;r;","%char;"a"%char;"_"%char;a;b;c;")"%char] => Some (InscribedAngle (circle_name o r) (angle_name a b c))
+  | ["r"%char;"e"%char;"f"%char;"_"%char;"s"%char;"e"%char;"g"%char;"("%char;a;b;","%char;c;d;")"%char] => Some (RefSeg (segment_name a b) (segment_name c d))
+  | ["r"%char;"e"%char;"f"%char;"_"%char;"a"%char;"n"%char;"g"%char;"("%char;"a"%char;"_"%char;a;b;c;","%char;"a"%char;"_"%char;d;e;f;")"%char] => Some (RefAng (angle_name a b c) (angle_name d e f))
+  | ["c"%char;"o"%char;"n"%char;"_"%char;"a"%char;"r"%char;"c"%char;"("%char;"m"%char;"i"%char;"n"%char;"o"%char;"r"%char;"_"%char;"a"%char;"r"%char;"c"%char;"("%char;"c"%char;"_"%char;o1;r1;","%char;a1;","%char;b1;")"%char;","%char;"m"%char;"i"%char;"n"%char;"o"%char;"r"%char;"_"%char;"a"%char;"r"%char;"c"%char;"("%char;"c"%char;"_"%char;o2;r2;","%char;a2;","%char;b2;")"%char;")"%char] => Some (ConArc (arc_name MinorArc (circle_name o1 r1) a1 b1) (arc_name MinorArc (circle_name o2 r2) a2 b2))
+  | ["c"%char;"o"%char;"n"%char;"_"%char;"a"%char;"r"%char;"c"%char;"("%char;"m"%char;"i"%char;"n"%char;"o"%char;"r"%char;"_"%char;"a"%char;"r"%char;"c"%char;"("%char;"c"%char;"_"%char;o1;r1;","%char;a1;","%char;b1;")"%char;","%char;"m"%char;"a"%char;"j"%char;"o"%char;"r"%char;"_"%char;"a"%char;"r"%char;"c"%char;"("%char;"c"%char;"_"%char;o2;r2;","%char;a2;","%char;b2;")"%char;")"%char] => Some (ConArc (arc_name MinorArc (circle_name o1 r1) a1 b1) (arc_name MajorArc (circle_name o2 r2) a2 b2))
+  | ["c"%char;"o"%char;"n"%char;"_"%char;"a"%char;"r"%char;"c"%char;"("%char;"m"%char;"a"%char;"j"%char;"o"%char;"r"%char;"_"%char;"a"%char;"r"%char;"c"%char;"("%char;"c"%char;"_"%char;o1;r1;","%char;a1;","%char;b1;")"%char;","%char;"m"%char;"i"%char;"n"%char;"o"%char;"r"%char;"_"%char;"a"%char;"r"%char;"c"%char;"("%char;"c"%char;"_"%char;o2;r2;","%char;a2;","%char;b2;")"%char;")"%char] => Some (ConArc (arc_name MajorArc (circle_name o1 r1) a1 b1) (arc_name MinorArc (circle_name o2 r2) a2 b2))
+  | ["c"%char;"o"%char;"n"%char;"_"%char;"a"%char;"r"%char;"c"%char;"("%char;"m"%char;"a"%char;"j"%char;"o"%char;"r"%char;"_"%char;"a"%char;"r"%char;"c"%char;"("%char;"c"%char;"_"%char;o1;r1;","%char;a1;","%char;b1;")"%char;","%char;"m"%char;"a"%char;"j"%char;"o"%char;"r"%char;"_"%char;"a"%char;"r"%char;"c"%char;"("%char;"c"%char;"_"%char;o2;r2;","%char;a2;","%char;b2;")"%char;")"%char] => Some (ConArc (arc_name MajorArc (circle_name o1 r1) a1 b1) (arc_name MajorArc (circle_name o2 r2) a2 b2))
+  | _ => None
+  end.
+
+Definition parse_public_statement_chars (text : PChars) : option PublicStatement :=
+  match parse_rendered_statement text with
+  | Some statement => Some statement
+  | None => parse_public_statement_chars_generic text
+  end.
+
 Definition parse_public_statement (text : string) : option PublicStatement :=
   let input := normalized text in
   match parse_public_statement_chars input with
   | Some statement =>
-      if chars_eqb input (list_ascii_of_string (statementText statement))
-      then Some statement else None
+      if pointsValid (statementPoints statement) then
+        if chars_eqb input (list_ascii_of_string (statementText statement))
+        then Some statement else None
+      else None
   | None => None
   end.
+
+Ltac solve_statement_render :=
+  repeat match goal with
+  | s : SegmentName |- _ => destruct s
+  | a : AngleName |- _ => destruct a
+  | t : TriangleName |- _ => destruct t
+  | q : QuadrilateralName |- _ => destruct q
+  | c : CircleName |- _ => destruct c
+  | a : ArcName |- _ => destruct a
+  | k : ArcKind |- _ => destruct k
+  end;
+  reflexivity.
+
+Lemma parse_public_statement_chars_render : forall statement,
+  pointsValid (statementPoints statement) = true ->
+  parse_public_statement_chars
+    (list_ascii_of_string (statementText statement)) = Some statement.
+Proof.
+  intros statement Hvalid. destruct statement.
+  all: abstract solve_statement_render.
+Qed.
+
+Theorem parse_public_statement_complete : forall text statement,
+  StatementText text statement -> parse_public_statement text = Some statement.
+Proof.
+  intros text statement [Hvalid Htext]. unfold parse_public_statement.
+  rewrite Htext, parse_public_statement_chars_render by exact Hvalid.
+  rewrite Hvalid, (proj2 (chars_eqb_eq _ _) eq_refl). reflexivity.
+Qed.
 
 Theorem parse_public_statement_sound : forall text statement,
   parse_public_statement text = Some statement -> StatementText text statement.
@@ -163,10 +252,12 @@ Proof.
   intros text statement H. unfold parse_public_statement in H.
   destruct (parse_public_statement_chars (normalized text)) as [parsed|] eqn:Hparsed;
     try discriminate.
+  destruct (pointsValid (statementPoints parsed)) eqn:Hvalid; cbn in H;
+    try discriminate.
   destruct (chars_eqb (normalized text)
              (list_ascii_of_string (statementText parsed))) eqn:Heq;
     try discriminate.
-  injection H as <-. now apply chars_eqb_eq in Heq.
+  injection H as <-. split; [exact Hvalid|]. now apply chars_eqb_eq in Heq.
 Qed.
 
 Fixpoint parse_segment_declarations (text : PChars) : option (list PublicDeclaration) :=
@@ -180,13 +271,97 @@ Fixpoint parse_quad_declarations (text : PChars) : option (list PublicDeclaratio
 Fixpoint parse_circle_declarations (text : PChars) : option (list PublicDeclaration) :=
   match text with []=>Some[] | "c"%char::"_"%char::o::r::rest => match parse_circle_declarations rest with Some ds=>Some(CircleDeclaration(circle_name o r)::ds)|_=>None end | _=>None end.
 
-Definition parse_declaration_line_raw (line : string) : option (list PublicDeclaration) :=
-  let text:=normalized line in
+Lemma concat_empty_cons : forall first rest,
+  String.concat "" (first :: rest) = first ++ String.concat "" rest.
+Proof. intros first rest. destruct rest; cbn; induction first; cbn; congruence. Qed.
+
+Lemma list_ascii_append : forall a b,
+  list_ascii_of_string (a ++ b) =
+  List.app (list_ascii_of_string a) (list_ascii_of_string b).
+Proof. induction a; cbn; intros; [reflexivity|now rewrite IHa]. Qed.
+
+Lemma parse_segment_declarations_render : forall declarations,
+  Forall (fun d => declarationTag d = "seg:") declarations ->
+  parse_segment_declarations
+    (list_ascii_of_string (String.concat "" (map declarationObjectText declarations))) =
+  Some declarations.
+Proof.
+  intros declarations H. induction H as [|d ds Hd Hds IH]; [reflexivity|].
+  cbn [map]. rewrite concat_empty_cons, list_ascii_append.
+  destruct d; cbn in Hd; try discriminate. destruct s. cbn. now rewrite IH.
+Qed.
+
+Lemma parse_angle_declarations_render : forall declarations,
+  Forall (fun d => declarationTag d = "ang:") declarations ->
+  parse_angle_declarations
+    (list_ascii_of_string (String.concat "" (map declarationObjectText declarations))) =
+  Some declarations.
+Proof.
+  intros declarations H. induction H as [|d ds Hd Hds IH]; [reflexivity|].
+  cbn [map]. rewrite concat_empty_cons, list_ascii_append.
+  destruct d; cbn in Hd; try discriminate. destruct a. cbn. now rewrite IH.
+Qed.
+
+Lemma parse_triangle_declarations_render : forall declarations,
+  Forall (fun d => declarationTag d = "tri:") declarations ->
+  parse_triangle_declarations
+    (list_ascii_of_string (String.concat "" (map declarationObjectText declarations))) =
+  Some declarations.
+Proof.
+  intros declarations H. induction H as [|d ds Hd Hds IH]; [reflexivity|].
+  cbn [map]. rewrite concat_empty_cons, list_ascii_append.
+  destruct d; cbn in Hd; try discriminate. destruct t. cbn. now rewrite IH.
+Qed.
+
+Lemma parse_quad_declarations_render : forall declarations,
+  Forall (fun d => declarationTag d = "quad:") declarations ->
+  parse_quad_declarations
+    (list_ascii_of_string (String.concat "" (map declarationObjectText declarations))) =
+  Some declarations.
+Proof.
+  intros declarations H. induction H as [|d ds Hd Hds IH]; [reflexivity|].
+  cbn [map]. rewrite concat_empty_cons, list_ascii_append.
+  destruct d; cbn in Hd; try discriminate. destruct q. cbn. now rewrite IH.
+Qed.
+
+Lemma parse_circle_declarations_render : forall declarations,
+  Forall (fun d => declarationTag d = "circ:") declarations ->
+  parse_circle_declarations
+    (list_ascii_of_string (String.concat "" (map declarationObjectText declarations))) =
+  Some declarations.
+Proof.
+  intros declarations H. induction H as [|d ds Hd Hds IH]; [reflexivity|].
+  cbn [map]. rewrite concat_empty_cons, list_ascii_append.
+  destruct d; cbn in Hd; try discriminate. destruct c. cbn. now rewrite IH.
+Qed.
+
+Definition parse_declaration_line_raw_chars (text : PChars)
+    : option (list PublicDeclaration) :=
   if ProblemPart.starts_with (list_ascii_of_string "seg:") text then parse_segment_declarations(ProblemPart.drop_chars 4 text) else
   if ProblemPart.starts_with (list_ascii_of_string "ang:") text then parse_angle_declarations(ProblemPart.drop_chars 4 text) else
   if ProblemPart.starts_with (list_ascii_of_string "tri:") text then parse_triangle_declarations(ProblemPart.drop_chars 4 text) else
   if ProblemPart.starts_with (list_ascii_of_string "quad:") text then parse_quad_declarations(ProblemPart.drop_chars 5 text) else
   if ProblemPart.starts_with (list_ascii_of_string "circ:") text then parse_circle_declarations(ProblemPart.drop_chars 5 text) else None.
+
+Definition parse_declaration_line_raw (line : string) : option (list PublicDeclaration) :=
+  parse_declaration_line_raw_chars (normalized line).
+
+Lemma parse_declaration_line_raw_chars_render : forall first rest,
+  Forall (fun declaration => declarationTag declaration = declarationTag first) rest ->
+  parse_declaration_line_raw_chars
+    (list_ascii_of_string (declarationTag first ++
+      String.concat "" (map declarationObjectText (first :: rest)))) =
+  Some (first :: rest).
+Proof.
+  intros first rest Htags. cbn [map].
+  rewrite concat_empty_cons, !list_ascii_append.
+  destruct first; cbn in Htags |- *.
+  - destruct s. cbn. now rewrite parse_segment_declarations_render by exact Htags.
+  - destruct a. cbn. now rewrite parse_angle_declarations_render by exact Htags.
+  - destruct t. cbn. now rewrite parse_triangle_declarations_render by exact Htags.
+  - destruct q. cbn. now rewrite parse_quad_declarations_render by exact Htags.
+  - destruct c. cbn. now rewrite parse_circle_declarations_render by exact Htags.
+Qed.
 
 Definition declarations_text (declarations : list PublicDeclaration) : option string :=
   match declarations with
@@ -199,17 +374,41 @@ Definition declarations_text (declarations : list PublicDeclaration) : option st
       else None
   end.
 
+Definition declarations_valid (declarations : list PublicDeclaration) : bool :=
+  forallb (fun declaration => pointsValid (declarationPoints declaration)) declarations.
+
 Definition parse_declaration_line (line : string) : option (list PublicDeclaration) :=
   match parse_declaration_line_raw line with
   | Some declarations =>
       match declarations_text declarations with
       | Some rendered =>
-          if chars_eqb (normalized line) (list_ascii_of_string rendered)
-          then Some declarations else None
+          if declarations_valid declarations then
+            if chars_eqb (normalized line) (list_ascii_of_string rendered)
+            then Some declarations else None
+          else None
       | None => None
       end
   | None => None
   end.
+
+Theorem parse_declaration_line_complete : forall line declarations,
+  DeclarationText line declarations ->
+  parse_declaration_line line = Some declarations.
+Proof.
+  intros line declarations
+    [first [rest [-> [Htags [Hvalid Htext]]]]].
+  unfold parse_declaration_line.
+  unfold parse_declaration_line_raw.
+  rewrite Htext.
+  rewrite parse_declaration_line_raw_chars_render by exact Htags.
+  unfold declarations_text.
+  rewrite (proj2 (forallb_forall _ _) (fun declaration Hin =>
+    proj2 (String.eqb_eq _ _)
+      (proj1 (Forall_forall _ _) Htags declaration Hin))).
+  unfold declarations_valid. rewrite (proj2 (forallb_forall _ _) (fun declaration Hin =>
+    proj1 (Forall_forall _ _) Hvalid declaration Hin)).
+  rewrite (proj2 (chars_eqb_eq _ _) eq_refl). reflexivity.
+Qed.
 
 Theorem parse_declaration_line_sound : forall line declarations,
   parse_declaration_line line = Some declarations ->
@@ -223,37 +422,44 @@ Proof.
   destruct (forallb (fun declaration =>
     String.eqb (declarationTag declaration) (declarationTag first)) rest)
     eqn:Htags; try discriminate.
+  destruct (declarations_valid (first :: rest))
+    eqn:Hvalid.
+  2: discriminate.
   destruct (chars_eqb (normalized line)
     (list_ascii_of_string
       (declarationTag first ++
        String.concat "" (map declarationObjectText (first :: rest)))))
     eqn:Heq; try discriminate.
-  injection H as <-. exists first, rest. split; [reflexivity|]. split.
+  cbn in Heq. injection H as <-.
+  exists first, rest. split; [reflexivity|]. split.
   - rewrite forallb_forall in Htags. apply Forall_forall. intros declaration Hin.
     specialize (Htags declaration Hin). now apply String.eqb_eq in Htags.
-  - now apply chars_eqb_eq in Heq.
+  - split.
+    + unfold declarations_valid in Hvalid. apply Forall_forall.
+      rewrite forallb_forall in Hvalid. exact Hvalid.
+    + now apply chars_eqb_eq in Heq.
 Qed.
 
 Definition HeaderContribution :=
   (list PublicDeclaration * list PublicStatement * option PublicStatement)%type.
 
 Definition parse_public_line (line : string) : option HeaderContribution :=
-  match parse_declaration_line line with
-  | Some declarations => Some (declarations, [], None)
+  match premiseBody line with
+  | Some body =>
+      match parse_public_statement body with
+      | Some statement => Some ([], [statement], None)
+      | None => None
+      end
   | None =>
-      match premiseBody line with
+      match goalBody line with
       | Some body =>
           match parse_public_statement body with
-          | Some statement => Some ([], [statement], None)
+          | Some statement => Some ([], [], Some statement)
           | None => None
           end
       | None =>
-          match goalBody line with
-          | Some body =>
-              match parse_public_statement body with
-              | Some statement => Some ([], [], Some statement)
-              | None => None
-              end
+          match parse_declaration_line line with
+          | Some declarations => Some (declarations, [], None)
           | None => if chars_eqb (normalized line) []
                     then Some ([], [], None) else None
           end
@@ -264,17 +470,33 @@ Theorem parse_public_line_sound : forall line contribution,
   parse_public_line line = Some contribution -> HeaderLine line contribution.
 Proof.
   intros line contribution H. unfold parse_public_line in H.
-  destruct (parse_declaration_line line) as [declarations|] eqn:Hdeclarations.
-  - injection H as <-. constructor. now apply parse_declaration_line_sound.
-  - destruct (premiseBody line) as [body|] eqn:Hpremise.
+  destruct (premiseBody line) as [body|] eqn:Hpremise.
+  - destruct (parse_public_statement body) as [statement|] eqn:Hstatement;
+      try discriminate. injection H as <-. econstructor; eauto using parse_public_statement_sound.
+  - destruct (goalBody line) as [body|] eqn:Hgoal.
     + destruct (parse_public_statement body) as [statement|] eqn:Hstatement;
         try discriminate. injection H as <-. econstructor; eauto using parse_public_statement_sound.
-    + destruct (goalBody line) as [body|] eqn:Hgoal.
-      * destruct (parse_public_statement body) as [statement|] eqn:Hstatement;
-          try discriminate. injection H as <-. econstructor; eauto using parse_public_statement_sound.
+    + destruct (parse_declaration_line line) as [declarations|] eqn:Hdeclarations.
+      * injection H as <-. constructor; eauto using parse_declaration_line_sound.
       * destruct (chars_eqb (normalized line) []) eqn:Hblank; try discriminate.
-        injection H as <-. apply IgnoredBlankLine.
+        injection H as <-. apply IgnoredBlankLine; try assumption.
         exact (proj1 (chars_eqb_eq _ _) Hblank).
+Qed.
+
+Theorem parse_public_line_complete : forall line contribution,
+  HeaderLine line contribution -> parse_public_line line = Some contribution.
+Proof.
+  intros line contribution H. inversion H; subst; unfold parse_public_line.
+  - rewrite H0, H1, (parse_declaration_line_complete line declarations H2).
+    reflexivity.
+  - rewrite H0, (parse_public_statement_complete body statement H1). reflexivity.
+  - rewrite H0, H1, (parse_public_statement_complete body statement H2).
+    reflexivity.
+  - rewrite H0, H1. destruct (parse_declaration_line line) eqn:Hdeclaration.
+    + exfalso. apply parse_declaration_line_sound in Hdeclaration.
+      destruct Hdeclaration as [first [rest [_ [_ [_ Htext]]]]].
+      rewrite H2 in Htext. destruct first; discriminate.
+    + rewrite (proj2 (chars_eqb_eq _ _) H2). reflexivity.
 Qed.
 
 Fixpoint parse_public_lines (lines : list string) : option HeaderContribution :=
@@ -323,6 +545,18 @@ Proof.
       * left; reflexivity.
 Qed.
 
+Theorem parse_public_lines_complete : forall lines declarations premises goal,
+  HeaderLines lines declarations premises goal ->
+  parse_public_lines lines = Some (declarations, premises, goal).
+Proof.
+  intros lines declarations premises goal H. induction H.
+  - reflexivity.
+  - cbn. rewrite (parse_public_line_complete line
+      (lineDeclarations, linePremises, lineGoal) H).
+    rewrite IHHeaderLines. destruct lineGoal, goal; cbn in *; try reflexivity.
+    destruct H1; discriminate.
+Qed.
+
 Definition parsePublicProblem (source:string) : option PublicProblem :=
   match parse_public_lines (splitLines source) with
   |Some (declarations, premises, Some goal) =>
@@ -338,4 +572,12 @@ Proof.
     eqn:Hlines; try discriminate.
   destruct goal as [conclusion|]; try discriminate. injection H as <-.
   constructor. now eapply parse_public_lines_sound.
+Qed.
+
+Theorem parsePublicProblem_complete : forall source problem,
+  ProblemGrammar source problem -> parsePublicProblem source = Some problem.
+Proof.
+  intros source problem H. inversion H; subst. unfold parsePublicProblem.
+  rewrite (parse_public_lines_complete (splitLines source) declarations premises
+    (Some conclusion) H0). reflexivity.
 Qed.
